enable Kinding judgements on Intermediate.GlobalEnv

Intermediate/Typing.lean
@@ -8,7 +8,38 @@ open Lilac
 namespace Intermediate
 
 
-def Query (G : List Global) (c : DataConst) (qs : Vec String m) (Ts : Vec Core.Ty m) : Prop :=
+def Query (G : GlobalEnv) (c : DataConst) (qs : Vec String m) (Ts : Vec Core.Ty m) : Prop :=
   VecTyping (lookup_ctor? G c · ·) qs Ts
+
+
+inductive Kinding (G : List Intermediate.Global) : List Core.Kind -> Core.Ty -> Core.Kind -> Prop
+| var :
+  Δ[x]? = some K ->
+  Kinding G Δ t#x K
+| global :
+  lookup_kind G x = some K ->
+  Kinding G Δ gt#x K
+| arrow :
+  Kinding G Δ A ★ ->
+  Kinding G Δ B ★ ->
+  Kinding G Δ (A -:> B) ★
+| all :
+  Kinding G (K::Δ) P ★ ->
+  Kinding G Δ (∀[K] P) ★
+| app :
+  Kinding G Δ f (A -:> B) ->
+  Kinding G Δ a A ->
+  Kinding G Δ (f • a) B
+| eq :
+  Kinding G Δ A K ->
+  Kinding G Δ B K ->
+  Kinding G Δ (A ~[K]~ B) ★
+
+notation:170 G:170 "&" Δ:170 " ⊢ " A:170 " : " K:170 => Kinding G Δ A K
+
+def Ty.data? (c : DataConst) (G : List Global) (A : Core.Ty) : Bool :=
+  match A.spine with
+  | some (x, _) => is_data c G x
+  | none => false
 
 end Intermediate
